ConcreteTransformerLemmas.v
@@ -23,6 +23,18 @@ Transparent map_from_ps.
 Transparent update_varlike.
 Transparent lookup_varlike.
 
+(* A ctrl lookup reads only the ctrl map, so two states with equal ctrl maps
+   agree on every ctrl lookup. *)
+Lemma lookup_varlike_ctrl_t_ctrl_map :
+  forall (c1 c2 : ConcreteTransformerState) (v : Ctrl),
+    t_ctrl_map c1 = t_ctrl_map c2 ->
+    lookup_varlike c1 v = lookup_varlike c2 v.
+Proof.
+  intros c1 c2 v H.
+  unfold lookup_varlike. cbn [map_from_ps CrVarLike_Ctrl].
+  rewrite H. reflexivity.
+Qed.
+
 (* update_varlike preserves cs_lookup_eq, regardless of the variable type.
 
    The cross-type cases (e.g. updating a Header doesn't affect State / Ctrl
@@ -69,11 +81,11 @@ Qed.
 (* lookup_concrete (used to evaluate function arguments) commutes with
    cs_lookup_eq. *)
 Lemma lookup_concrete_eq :
-  forall c1 c2 arg,
+  forall c1 c2 ty arg,
   cs_lookup_eq c1 c2 ->
-  lookup_concrete arg c1 = lookup_concrete arg c2.
+  lookup_concrete ty arg c1 = lookup_concrete ty arg c2.
 Proof.
-  intros c1 c2 arg [Hh [Hs Hc]]. destruct arg; simpl;
+  intros c1 c2 ty arg [Hh [Hs Hc]]. destruct arg; simpl;
     [apply Hc | apply Hh | reflexivity | apply Hs].
 Qed.
 
@@ -84,7 +96,7 @@ Lemma eval_hdr_op_expr_concrete_eq :
 Proof.
   intros c1 c2 op Hcs.
   destruct op; cbn [eval_hdr_op_expr_concrete];
-    rewrite !(lookup_concrete_eq _ _ _ Hcs); reflexivity.
+    rewrite !(lookup_concrete_eq _ _ _ _ Hcs); reflexivity.
 Qed.
 
 Lemma eval_match_concrete_eq :
